\newproblem{20a}
{
	Find the distance between $(3, -6)$ and $(-1,-9)$.
}
{
	\begin{tabular}{l r}
	$d=\sqrt{(-1-3)^2+(-9-(-6))^2}$ & \\
	$d=\sqrt{(-4)^2+(-3)^2}$ & 1 pts to here\\
	$d=\sqrt{16+9}$ & 2 pts to here\\
	$d=\sqrt{25}$ & 3 pts to here\\
	$d=5$ & 4 pts to here
	\end{tabular}
}

\newproblem{20b}
{
	Find the distance between $(1, -3)$ and $(-11,-8)$.
}
{
	\begin{tabular}{l r}
	$d=\sqrt{(1-(-11))^2+(-3-(-8))^2}$ & \\
	$d=\sqrt{(12)^2+(5)^2}$ & 1 pts to here\\
	$d=\sqrt{144+25}$ & 2 pts to here\\
	$d=\sqrt{169}$ & 3 pts to here\\
	$d=13$ & 4 pts to here
	\end{tabular}
}

\newproblem{20c}
{
	Find the distance between $(4, -5)$ and $(-2,-13)$.
}
{
	\begin{tabular}{l r}
	$d=\sqrt{(4-(-2))^2+(-5-(-13))^2}$ & \\
	$d=\sqrt{(6)^2+(8)^2}$ & 1 pts to here\\
	$d=\sqrt{36+64}$ & 2 pts to here\\
	$d=\sqrt{100}$ & 3 pts to here\\
	$d=10$ & 4 pts to here
	\end{tabular}
}

\newproblem{20d}
{
	Find the distance between $(-7, 13)$ and $(-12,1)$.
}
{
	\begin{tabular}{l r}
	$d=\sqrt{(-7-(-12))^2+(13-1)^2}$ & \\
	$d=\sqrt{(5)^2+(12)^2}$ & 1 pts to here\\
	$d=\sqrt{25+144}$ & 2 pts to here\\
	$d=\sqrt{169}$ & 3 pts to here\\
	$d=13$ & 4 pts to here
	\end{tabular}
}
